examples/lambda/other-models/MPlambdaScript.sml
@@ -142,25 +142,34 @@ val vsub_14a = Store_thm(
   Induct THEN SRW_TAC [][]);
 
 
-val MPpm_def = Define`
-  (MPpm pi (Parameter s) = Parameter (lswapstr pi s)) /\
-  (MPpm pi (Var v) = Var v) /\
-  (MPpm pi (App t1 t2) = App (MPpm pi t1) (MPpm pi t2)) /\
-  (MPpm pi (Abs v t) = Abs v (MPpm pi t))
+val raw_MPpm_def = Define`
+  (raw_MPpm pi (Parameter s) = Parameter (lswapstr pi s)) /\
+  (raw_MPpm pi (Var v) = Var v) /\
+  (raw_MPpm pi (App t1 t2) = App (raw_MPpm pi t1) (raw_MPpm pi t2)) /\
+  (raw_MPpm pi (Abs v t) = Abs v (raw_MPpm pi t))
 `;
-val _ = export_rewrites ["MPpm_def"]
+val _ = export_rewrites ["raw_MPpm_def"]
 
 val lswapstr_APPEND = basic_swapTheory.lswapstr_APPEND
 
-val MPpm_is_perm = Store_thm(
-  "MPpm_is_perm",
-  ``is_perm MPpm``,
-  SRW_TAC [][is_perm_def] THENL [
+val _ = overload_on("MP_pmact",``mk_pmact raw_MPpm``);
+val _ = overload_on("MPpm", ``pmact MP_pmact``);
+
+val MPpm_raw = store_thm(
+  "MPpm_raw",
+  ``MPpm = raw_MPpm``,
+  SRW_TAC [][GSYM pmact_bijections] THEN
+  SRW_TAC [][is_pmact_def] THENL [
     Induct_on `x` THEN SRW_TAC [][],
     Induct_on `x` THEN SRW_TAC [][lswapstr_APPEND],
     FULL_SIMP_TAC (srw_ss()) [permeq_def, FUN_EQ_THM] THEN
     Induct THEN SRW_TAC [][]
   ]);
+
+val MPpm_thm = save_thm(
+"MPpm_thm",
+raw_MPpm_def |> SUBS [GSYM MPpm_raw, GSYM stringpm_raw]);
+val _ = export_rewrites["MPpm_thm"];
 
 val MPpm_fresh = Store_thm(
   "MPpm_fresh",
@@ -175,7 +184,7 @@ val MPpm_NIL = Store_thm(
 
 val supp_MPpm = Store_thm(
   "supp_MPpm",
-  ``supp MPpm = params``,
+  ``supp MP_pmact = params``,
   ONCE_REWRITE_TAC [FUN_EQ_THM] THEN GEN_TAC THEN
   MATCH_MP_TAC supp_unique_apart THEN SRW_TAC [][support_def] THEN
   Induct_on `x` THEN SRW_TAC [][] THEN METIS_TAC []);
@@ -257,7 +266,7 @@ val IN_params_MPpm = store_thm(
   "IN_params_MPpm",
   ``x IN params (MPpm pi M) = lswapstr (REVERSE pi) x IN params M``,
   Induct_on `M` THEN SRW_TAC [][] THEN
-  SRW_TAC [][basic_swapTheory.lswapstr_eqr]);
+  SRW_TAC [][basic_swapTheory.lswapstr_eqr, stringpm_raw]);
 
 val independent_psub_vsub = prove(
   ``!M v p1 p2 p3.
@@ -301,11 +310,11 @@ val cvclosed_strongctxt_ind = prove(
   FULL_SIMP_TAC (srw_ss()) [MPpm_vsub] THEN
   Q_TAC (NEW_TAC "z") `f x UNION params (MPpm pi M)` THEN
   Q.EXISTS_TAC `z` THEN SRW_TAC [][] THEN
-  FIRST_X_ASSUM (Q.SPECL_THEN [`(lswapstr pi p, z) :: pi`, `x'`] MP_TAC) THEN
+  FIRST_X_ASSUM (Q.SPECL_THEN [`(stringpm pi p, z) :: pi`, `x'`] MP_TAC) THEN
   ASM_SIMP_TAC (srw_ss()) [] THEN
-  `MPpm [(lswapstr pi p, z)] (MPpm pi M) = MPpm pi M`
-    by SRW_TAC [][MPpm_fresh, IN_params_MPpm] THEN
-  FULL_SIMP_TAC (srw_ss()) [GSYM is_perm_decompose]);
+  `MPpm [(stringpm pi p, z)] (MPpm pi M) = MPpm pi M`
+    by SRW_TAC [][MPpm_fresh, IN_params_MPpm, stringpm_raw] THEN
+  FULL_SIMP_TAC (srw_ss()) [GSYM pmact_decompose]);
 
 val cvclosed_strong_ind =
 (Q.GEN `P` o Q.GEN `X` o
@@ -392,13 +401,13 @@ val cofin_vclosed_ind = store_thm(
   Q.EXISTS_TAC `params (MPpm pi t)` THEN
   FULL_SIMP_TAC (srw_ss()) [MPpm_vsub] THEN
   Q.X_GEN_TAC `p1` THEN STRIP_TAC THEN
-  FIRST_X_ASSUM (Q.SPEC_THEN `[(p1,lswapstr pi p)] ++ pi` MP_TAC) THEN
+  FIRST_X_ASSUM (Q.SPEC_THEN `[(p1,stringpm pi p)] ++ pi` MP_TAC) THEN
   ASM_SIMP_TAC (srw_ss()) [] THEN
-  Q_TAC SUFF_TAC `MPpm ((p1,lswapstr pi p)::pi) t = MPpm pi t`
+  Q_TAC SUFF_TAC `MPpm ((p1,stringpm pi p)::pi) t = MPpm pi t`
         THEN1 SRW_TAC [][] THEN
-  `MPpm [(p1,lswapstr pi p)] (MPpm pi t) = MPpm pi t`
-     by SRW_TAC [][MPpm_fresh, IN_params_MPpm] THEN
-  FULL_SIMP_TAC (srw_ss()) [GSYM is_perm_decompose]);
+  `MPpm [(p1,stringpm pi p)] (MPpm pi t) = MPpm pi t`
+     by SRW_TAC [][MPpm_fresh, IN_params_MPpm, stringpm_raw] THEN
+  FULL_SIMP_TAC (srw_ss()) [GSYM pmact_decompose]);
 
 val (avclosed_rules, avclosed_ind, avclosed_cases) = Hol_reln`
   (!p. avclosed (Parameter p)) /\
@@ -557,15 +566,14 @@ val params_vsub = store_thm(
 val convert_MPpm = prove(
   ``!t M. convert t M ==> !pi. convert (MPpm pi t) (tpm pi M)``,
   HO_MATCH_MP_TAC convert_ind THEN
-  SRW_TAC [][convert_rules, MPpm_vsub] THEN
+  SRW_TAC [][convert_rules, MPpm_vsub, stringpm_raw] THEN
   MATCH_MP_TAC (last (CONJUNCTS convert_rules)) THEN
   SRW_TAC [][IN_params_MPpm]);
 
 val convert_MPpm_E = Store_thm(
   "convert_MPpm_E",
   ``convert (MPpm pi t) (tpm pi M) = convert t M``,
-  METIS_TAC [convert_MPpm, is_perm_inverse, MPpm_is_perm,
-             termTheory.tpm_is_perm]);
+  METIS_TAC [convert_MPpm, pmact_inverse]);
 
 val convert_strong_ind = store_thm(
   "convert_strong_ind",
@@ -585,15 +593,15 @@ val convert_strong_ind = store_thm(
   Q_TAC SUFF_TAC `!t M. convert t M ==>
                         convert t M /\
                         !c pi. P (MPpm pi t) (tpm pi M) c`
-        THEN1 METIS_TAC [termTheory.tpm_NIL, MPpm_NIL] THEN
+        THEN1 METIS_TAC [pmact_nil] THEN
   HO_MATCH_MP_TAC convert_ind THEN
-  SRW_TAC [][convert_rules, MPpm_vsub] THEN
+  SRW_TAC [][convert_rules, MPpm_vsub, stringpm_raw] THEN
   Q_TAC (NEW_TAC "z") `FV (tpm pi M) UNION f c UNION params (MPpm pi t)` THEN
   `LAM (lswapstr pi u) (tpm pi M) = LAM z (tpm [(z, lswapstr pi u)] (tpm pi M))`
      by SRW_TAC [][termTheory.tpm_ALPHA] THEN
   SRW_TAC [][] THEN
   `MPpm ((z,lswapstr pi u)::pi) t = MPpm [(z,lswapstr pi u)] (MPpm pi t)`
-     by SRW_TAC [][GSYM is_perm_decompose] THEN
+     by SRW_TAC [][GSYM pmact_decompose] THEN
   ` _ = MPpm pi t`
      by SRW_TAC [][MPpm_fresh, IN_params_MPpm] THEN
   FIRST_X_ASSUM MATCH_MP_TAC THEN SRW_TAC [][]
@@ -602,9 +610,9 @@ val convert_strong_ind = store_thm(
               by METIS_TAC [convert_MPpm_E] THEN
            POP_ASSUM MP_TAC THEN
            ASM_SIMP_TAC bool_ss [MPpm_vsub] THEN
-           SRW_TAC [][GSYM termTheory.tpm_APPEND]) THEN
+           SRW_TAC [][GSYM pmact_decompose, stringpm_raw]) THEN
   FIRST_X_ASSUM (Q.SPECL_THEN [`d`, `((z,lswapstr pi u)::pi)`] MP_TAC) THEN
-  SRW_TAC [][GSYM termTheory.tpm_APPEND]);
+  SRW_TAC [][GSYM pmact_decompose]);
 
 val convert_params = store_thm(
   "convert_params",
@@ -685,7 +693,7 @@ val convert_unique = store_thm(
     `FV M' = params (vsub (Parameter u') v t)`
       by METIS_TAC [convert_params] THEN
     SRW_TAC [][notin_pvsub_I] THEN
-    METIS_TAC [convert_vsub_thm, termTheory.tpm_flip_args]
+    METIS_TAC [convert_vsub_thm, pmact_flip_args]
   ]);
 
 val convert_onto = store_thm(
@@ -783,7 +791,7 @@ val mpbeta_MPpm = prove(
   HO_MATCH_MP_TAC mpbeta_ind THEN
   SRW_TAC [][mpbeta_rules, MPpm_vsub] THENL [
     MATCH_MP_TAC (List.nth(CONJUNCTS mpbeta_rules, 2)) THEN
-    Q.EXISTS_TAC `lswapstr pi p` THEN SRW_TAC [][IN_params_MPpm],
+    Q.EXISTS_TAC `stringpm pi p` THEN SRW_TAC [][IN_params_MPpm, stringpm_raw],
     MATCH_MP_TAC (last (CONJUNCTS mpbeta_rules)) THEN
     `MPpm pi (Abs x M) = Abs x (MPpm pi M)` by SRW_TAC [][] THEN
     METIS_TAC [vclosed_MPpm]
@@ -806,8 +814,8 @@ val mpbeta_ccbeta = store_thm(
       SRW_TAC [][] THEN
       `convert (vsub (Parameter p) u M) (tpm [(p,u')] M'') /\
        convert (vsub (Parameter p) v N) (tpm [(p,u')] M''')`
-         by METIS_TAC [convert_vsub_thm, termTheory.tpm_flip_args] THEN
-      METIS_TAC [cc_beta_tpm_eqn, termTheory.tpm_inverse],
+         by METIS_TAC [convert_vsub_thm, pmact_flip_args] THEN
+      METIS_TAC [cc_beta_tpm_eqn, pmact_inverse],
       `~(u' IN FV M''')`
         by (`FV M''' = params (vsub (Parameter u'') v N)`
                by SRW_TAC [][convert_params] THEN
@@ -828,12 +836,12 @@ val mpbeta_ccbeta = store_thm(
       `compat_closure beta (tpm [(u',p)] M'') (tpm [(u'',p)] M''')`
          by METIS_TAC [] THEN
       `compat_closure beta M'' (tpm [(u',p)] (tpm [(u'',p)] M'''))`
-         by METIS_TAC [cc_beta_tpm, termTheory.tpm_sing_inv] THEN
+         by METIS_TAC [cc_beta_tpm, pmact_sing_inv] THEN
       Q_TAC SUFF_TAC `tpm [(u',p)] (tpm [(u'',p)] M''') = tpm [(u'',u')] M'''`
             THEN1 METIS_TAC [] THEN
       Cases_on `p = u'` THEN1 SRW_TAC [][] THEN
-      Cases_on `p = u''` THEN1 SRW_TAC [][termTheory.tpm_flip_args] THEN
-      ONCE_REWRITE_TAC [GSYM termTheory.tpm_sing_to_back] THEN
+      Cases_on `p = u''` THEN1 SRW_TAC [][pmact_flip_args] THEN
+      ONCE_REWRITE_TAC [GSYM pmact_sing_to_back] THEN
       SRW_TAC [][] THEN
       `~(p IN FV M''') /\ ~(u' IN FV M''')`
         by METIS_TAC [convert_params, notin_pvsub_I] THEN
@@ -875,8 +883,8 @@ val convert_to_lam = prove(
   SRW_TAC [boolSimps.DNF_ss][termTheory.LAM_eq_thm, termTheory.tpm_eqr] THEN
   SRW_TAC [][EQ_IMP_THM] THEN
   Q_TAC SUFF_TAC `~(v IN params t')`
-        THEN1 METIS_TAC [convert_vsub_thm, termTheory.tpm_flip_args,
-                         termTheory.tpm_sing_inv] THEN
+        THEN1 METIS_TAC [convert_vsub_thm, pmact_flip_args,
+                         pmact_sing_inv] THEN
   `~(v IN FV (tpm [(v,u)] M))` by SRW_TAC [][] THEN
   `~(v IN params (vsub (Parameter u) v' t'))`
     by METIS_TAC [convert_params] THEN
