examples/lambda/other-models/pure_dBScript.sml
@@ -2,7 +2,7 @@ open HolKernel boolLib Parse bossLib pred_setTheory termTheory BasicProvers
 
 open arithmeticTheory boolSimps
 
-local open string_numTheory in end
+local open string_numTheory chap2Theory chap3Theory in end
 
 fun Store_thm(trip as (n,t,tac)) = store_thm trip before export_rewrites [n]
 
@@ -140,18 +140,21 @@ val inc_pm_permeq = store_thm(
                        FUN_EQ_THM]);
 
 (* definition of permutation over de Bruijn terms *)
-val dpm_def = Define`
-  (dpm pi (dV i) = dV (s2n (lswapstr pi (n2s i)))) /\
-  (dpm pi (dAPP t u) = dAPP (dpm pi t) (dpm pi u)) /\
-  (dpm pi (dABS t) = dABS (dpm (inc_pm 0 pi) t))
+val raw_dpm_def = Define`
+  (raw_dpm pi (dV i) = dV (s2n (lswapstr pi (n2s i)))) /\
+  (raw_dpm pi (dAPP t u) = dAPP (raw_dpm pi t) (raw_dpm pi u)) /\
+  (raw_dpm pi (dABS t) = dABS (raw_dpm (inc_pm 0 pi) t))
 `;
-val _ = export_rewrites ["dpm_def"]
+val _ = export_rewrites ["raw_dpm_def"]
+val _ = overload_on("d_pmact",``mk_pmact raw_dpm``);
+val _ = overload_on("dpm",``pmact d_pmact``);
 
 (* proof that dB terms + dpm form a nominal set *)
-val dpm_is_perm = store_thm(
-  "dpm_is_perm",
-  ``is_perm dpm``,
-  SIMP_TAC (srw_ss()) [nomsetTheory.is_perm_def] THEN REPEAT CONJ_TAC THENL [
+val dpm_raw = store_thm(
+  "dpm_raw",
+  ``dpm = raw_dpm``,
+  SRW_TAC [][GSYM nomsetTheory.pmact_bijections] THEN
+  SIMP_TAC (srw_ss()) [nomsetTheory.is_pmact_def] THEN REPEAT CONJ_TAC THENL [
     Induct_on `x` THEN SRW_TAC [][],
     Induct_on `x` THEN SRW_TAC [][basic_swapTheory.lswapstr_APPEND,
                                   inc_pm_APPEND],
@@ -159,19 +162,12 @@ val dpm_is_perm = store_thm(
                          nomsetTheory.permeq_def] THEN
     Induct_on `x` THEN SRW_TAC [][lswapstr_inc_pm]
   ]);
-val _ = export_rewrites ["dpm_is_perm"]
+val dpm_thm = save_thm(
+"dpm_thm",
+raw_dpm_def |> SUBS [GSYM dpm_raw, GSYM nomsetTheory.stringpm_raw]);
+val _ = export_rewrites ["dpm_thm"]
 
 (* being a nominal set gives us properties of dpm "for free" *)
-val dpm_flip_args = store_thm(
-  "dpm_flip_args",
-  ``dpm ((x,y)::pi) t = dpm ((y,x)::pi) t``,
-  SRW_TAC [][nomsetTheory.is_perm_flip_args]);
-
-val dpm_sing_inv = store_thm(
-  "dpm_sing_inv",
-  ``dpm [h] (dpm [h] t) = t``,
-  SRW_TAC [][nomsetTheory.is_perm_sing_inv]);
-val _ = export_rewrites ["dpm_sing_inv"]
 
 (* dFVs gives the free indices of a dB term as strings *)
 val dFVs_def = Define`dFVs t = IMAGE n2s (dFV t)`
@@ -216,7 +212,7 @@ val dpm_fresh = store_thm(
 
 val dpm_supp = store_thm(
   "dpm_supp",
-  ``supp dpm = dFVs``,
+  ``supp d_pmact = dFVs``,
   ONCE_REWRITE_TAC [FUN_EQ_THM] THEN SRW_TAC [][] THEN
   MATCH_MP_TAC nomsetTheory.supp_unique_apart THEN
   SRW_TAC [][dpm_apart, nomsetTheory.support_def] THEN
@@ -232,9 +228,8 @@ val _ = binderLib.type_db :=
                          binderLib.NTI {
                          nullfv = ``dABS (dV 0)``,
                          pm_rewrites = [],
-                         pm_constant = ``dpm``,
+                         pm_constant = ``d_pmact``,
                          fv_rewrites = [],
-                         fv_constant = ``dFV``,
                          recursion_thm = NONE,
                          binders = []})
 
@@ -252,11 +247,13 @@ val inc_pm_0n = prove(
   ``!pi. inc_pm 0 (inc_pm n pi) = inc_pm (n + 1) (inc_pm 0 pi)``,
   Induct THEN ASM_SIMP_TAC (srw_ss()) [pairTheory.FORALL_PROD, ginc_0n])
 
+val stringpm_raw = nomsetTheory.stringpm_raw
+
 (* interaction of lifting and permutation *)
 val lift_dpm = store_thm(
   "lift_dpm",
   ``!n pi. lift (dpm pi M) n = dpm (inc_pm n pi) (lift M n)``,
-  Induct_on `M` THEN SRW_TAC [][lswapstr_inc_pm] THENL [
+  Induct_on `M` THEN SRW_TAC [][lswapstr_inc_pm,stringpm_raw] THENL [
     SRW_TAC [][ginc_def],
     ASM_SIMP_TAC (srw_ss() ++ ARITH_ss) [] THEN
     SRW_TAC [][ginc_def],
@@ -271,14 +268,14 @@ val dpm_sub = store_thm(
   ``!pi M j N.
         dpm pi (sub M j N) = sub (dpm pi M) (s2n (lswapstr pi (n2s j)))
                                          (dpm pi N)``,
-  Induct_on `N` THEN SRW_TAC [][lswapstr_inc_pm, lift_dpm] THEN
+  Induct_on `N` THEN SRW_TAC [][lswapstr_inc_pm, lift_dpm, stringpm_raw] THEN
   SRW_TAC [][ginc_0]);
 
 (* thus, so too is dLAM *)
 val dpm_dLAM = store_thm(
   "dpm_dLAM",
   ``dpm pi (dLAM j t) = dLAM (s2n (lswapstr pi (n2s j))) (dpm pi t)``,
-  SRW_TAC [][dLAM_def, dpm_sub, lift_dpm, lswapstr_inc_pm] THEN
+  SRW_TAC [][dLAM_def, dpm_sub, lift_dpm, lswapstr_inc_pm, stringpm_raw] THEN
   SRW_TAC [][ginc_0])
 val _ = export_rewrites ["dpm_dLAM"]
 
@@ -462,7 +459,7 @@ val fromTerm_eqlam = prove(
     SRW_TAC [][fromTerm_def, dLAM_def] THEN
     Cases_on `i = s2n v` THENL [
       FULL_SIMP_TAC (srw_ss()) [LAM_eq_thm, fresh_dpm_sub,
-                               nomsetTheory.is_perm_injective, lift_11],
+                               nomsetTheory.pmact_injective, lift_11],
       `~(i IN dFV (fromTerm t0)) /\ ~(s2n v IN dFV d)`
          by (FIRST_X_ASSUM (MP_TAC o AP_TERM ``dFV``) THEN
              REWRITE_TAC [EXTENSION] THEN
@@ -472,7 +469,7 @@ val fromTerm_eqlam = prove(
       FIRST_X_ASSUM (MP_TAC o AP_TERM ``dpm [(n2s 0, n2s (i + 1))]``) THEN
       ASM_SIMP_TAC (srw_ss()) [fresh_dpm_sub] THEN
       ASM_SIMP_TAC (srw_ss()) [GSYM fresh_dpm_sub] THEN
-      ONCE_REWRITE_TAC [dpm_flip_args] THEN
+      ONCE_REWRITE_TAC [nomsetTheory.pmact_flip_args] THEN
       `~(i + 1 IN dFV (sub (dV 0) (s2n v + 1) (lift (fromTerm t0) 0)))`
          by (SRW_TAC [ARITH_ss][dFVs_sub, IN_dFV] THEN
              SRW_TAC [][dFVs_def]) THEN
@@ -485,7 +482,7 @@ val fromTerm_eqlam = prove(
       SRW_TAC [][] THEN ONCE_REWRITE_TAC [GSYM fromTerm_tpm] THEN
       Q.EXISTS_TAC `tpm [(n2s i,v)] t0` THEN
       SRW_TAC [][LAM_eq_thm, sn_iso_num] THEN
-      FULL_SIMP_TAC (srw_ss()) [IN_dFV, tpm_flip_args]
+      FULL_SIMP_TAC (srw_ss()) [IN_dFV, nomsetTheory.pmact_flip_args]
     ],
     SRW_TAC [][] THEN SRW_TAC [][fromTerm_def]
   ])
@@ -653,7 +650,7 @@ val dbeta'_dpm = prove(
 val dbeta'_dpm_calc = store_thm(
   "dbeta'_dpm_calc",
   ``!M N. dbeta' (dpm pi M) N = dbeta' M (dpm (REVERSE pi) N)``,
-  METIS_TAC [dbeta'_dpm, nomsetTheory.is_perm_inverse, dpm_is_perm])
+  METIS_TAC [dbeta'_dpm, nomsetTheory.pmact_inverse])
 
 (* We can construct a lift permutation.
      inc_as_pm lim n
@@ -720,7 +717,7 @@ val lifts_are_specific_dpms = store_thm(
   ``!M n. (!i. i IN dFV M ==> i <= n) ==>
           !m. lift M m = dpm (lifting_pm m n) M``,
   Induct THEN SRW_TAC [][] THENL [
-    SRW_TAC [][lifting_pm_behaves],
+    SRW_TAC [][lifting_pm_behaves, stringpm_raw],
     FULL_SIMP_TAC (srw_ss() ++ DNF_ss) [inc_pm0_lifting_pm] THEN
     FIRST_X_ASSUM MATCH_MP_TAC THEN SRW_TAC [][] THEN
     Cases_on `i` THENL [
@@ -786,7 +783,7 @@ val dbeta'_lift = store_thm(
      by (CONJ_TAC THEN MATCH_MP_TAC lifts_are_specific_dpms THEN
          REPEAT STRIP_TAC THEN RES_TAC THEN Q.UNABBREV_TAC `k` THEN
          DECIDE_TAC) THEN
-  SRW_TAC [][dbeta'_dpm_calc, nomsetTheory.is_perm_inverse])
+  SRW_TAC [][dbeta'_dpm_calc, nomsetTheory.pmact_inverse])
 
 val dbeta_dbeta' = store_thm(
   "dbeta_dbeta'",
@@ -795,7 +792,7 @@ val dbeta_dbeta' = store_thm(
     SRW_TAC [][alt_dbeta'_rule],
     Q_TAC SUFF_TAC `!p t u. dbeta' (dpm p t) (dpm p u) = dbeta' t u`
           THEN1 METIS_TAC [dABS_rules_are_dLAM_compatible, dbeta'_rules] THEN
-    SRW_TAC [][dbeta'_dpm_calc, nomsetTheory.is_perm_inverse]
+    SRW_TAC [][dbeta'_dpm_calc, nomsetTheory.pmact_inverse]
   ]);
 
 (* nsub must be icky - just look at how it behaves under permutations *)
@@ -809,17 +806,17 @@ val dpm_nsub = store_thm(
       `lswapstr (inc_pm i pi) (n2s n) = ginc i (lswapstr pi (n2s (n - 1)))`
          by (SRW_TAC [][lswapstr_inc_pm] THEN
              FULL_SIMP_TAC (srw_ss() ++ ARITH_ss) []) THEN
-      ASM_SIMP_TAC (srw_ss()) [] THEN
+      ASM_SIMP_TAC (srw_ss()) [stringpm_raw] THEN
       Q.ABBREV_TAC `s = lswapstr pi (n2s (n - 1))` THEN
       SRW_TAC [][ginc_def] THEN FULL_SIMP_TAC (srw_ss() ++ ARITH_ss) [] THEN
       Cases_on `s2n s < i` THEN FULL_SIMP_TAC (srw_ss() ++ ARITH_ss) [],
 
       ASM_SIMP_TAC (srw_ss()) [] THEN Cases_on `i = n` THENL [
         ASM_SIMP_TAC (srw_ss()) [] THEN
-        SRW_TAC [][lswapstr_inc_pm],
+        SRW_TAC [][lswapstr_inc_pm, stringpm_raw],
         `lswapstr (inc_pm i pi) (n2s n) = ginc i (lswapstr pi (n2s n))`
            by SRW_TAC [ARITH_ss][lswapstr_inc_pm] THEN
-        ASM_SIMP_TAC (srw_ss()) [] THEN
+        ASM_SIMP_TAC (srw_ss()) [stringpm_raw] THEN
         Q.ABBREV_TAC `s = lswapstr pi (n2s n)` THEN
         SRW_TAC [][ginc_def] THEN FULL_SIMP_TAC (srw_ss() ++ ARITH_ss) [] THEN
         Cases_on `s2n s < i` THEN FULL_SIMP_TAC (srw_ss() ++ ARITH_ss) []
@@ -850,7 +847,7 @@ val dbeta_lift = store_thm(
      by (CONJ_TAC THEN MATCH_MP_TAC lifts_are_specific_dpms THEN
          REPEAT STRIP_TAC THEN RES_TAC THEN Q.UNABBREV_TAC `k` THEN
          DECIDE_TAC) THEN
-  METIS_TAC [dbeta_dpm, nomsetTheory.is_perm_inverse, dpm_is_perm])
+  METIS_TAC [dbeta_dpm, nomsetTheory.pmact_inverse])
 
 val dbeta'_dbeta = store_thm(
   "dbeta'_dbeta",
@@ -858,7 +855,7 @@ val dbeta'_dbeta = store_thm(
   HO_MATCH_MP_TAC dbeta'_ind THEN
   SRW_TAC [][dbeta_rules, alt_dbeta_rule] THEN
   METIS_TAC [dABS_rules_are_dLAM_compatible, dbeta_rules, dbeta_dpm,
-             nomsetTheory.is_perm_inverse, dpm_is_perm]);
+             nomsetTheory.pmact_inverse]);
 
 val dbeta_dbeta'_eqn = store_thm(
   "dbeta_dbeta'_eqn",
@@ -1112,9 +1109,9 @@ val IN_dFV_dpm = store_thm(
   "IN_dFV_dpm",
   ``!t p i. i IN dFV (dpm p t) = s2n (lswapstr (REVERSE p) (n2s i)) IN dFV t``,
   SRW_TAC [][IN_dFV] THEN REWRITE_TAC [SYM dpm_supp] THEN
-  `supp dpm (dpm p t) = setpm lswapstr p (supp dpm t)`
-     by METIS_TAC [nomsetTheory.perm_supp, dpm_is_perm] THEN
-  SRW_TAC [][]);
+  `supp d_pmact (dpm p t) = ssetpm p (supp d_pmact t)`
+     by METIS_TAC [nomsetTheory.perm_supp] THEN
+  SRW_TAC [][stringpm_raw]);
 
 val REVERSE_inc_pm = store_thm(
   "REVERSE_inc_pm",
@@ -1130,7 +1127,7 @@ val nipkow_eta_lemma = store_thm(
 val neta_dpm = store_thm(
   "neta_dpm",
   ``!t u. neta t u ==> !p. neta (dpm p t) (dpm p u)``,
-  HO_MATCH_MP_TAC neta_ind THEN SRW_TAC [][neta_rules] THEN
+  HO_MATCH_MP_TAC neta_ind THEN SRW_TAC [][neta_rules,stringpm_raw] THEN
   SRW_TAC [][lswapstr_inc_pm] THEN
   Q.MATCH_ABBREV_TAC `neta (dABS (dAPP tm (dV 0))) tm'` THEN
   Q_TAC SUFF_TAC `~(0 IN dFV tm) /\ (tm' = nsub u 0 tm)`
@@ -1155,7 +1152,7 @@ val eta_neta = store_thm(
   HO_MATCH_MP_TAC eta_ind THEN
   SRW_TAC [][neta_rules, alt_neta_redex] THEN
   METIS_TAC [neta_rules, dABS_rules_are_dLAM_compatible, neta_dpm,
-             nomsetTheory.is_perm_inverse, dpm_is_perm]);
+             nomsetTheory.pmact_inverse]);
 
 val nipkow_free_sub_lemmma = store_thm(
   "nipkow_free_sub_lemmma",
@@ -1173,14 +1170,14 @@ val lift_nsub = store_thm(
 val eta_dpm = store_thm(
   "eta_dpm",
   ``!t u. eta t u ==> !p. eta (dpm p t) (dpm p u)``,
-  HO_MATCH_MP_TAC eta_ind THEN SRW_TAC [][eta_rules] THEN
+  HO_MATCH_MP_TAC eta_ind THEN SRW_TAC [][eta_rules,stringpm_raw] THEN
   MATCH_MP_TAC (hd (CONJUNCTS eta_rules)) THEN
   SRW_TAC [][IN_dFV_dpm]);
 
 val eta_dpm_eqn = store_thm(
   "eta_dpm_eqn",
   ``eta (dpm p t) (dpm p u) = eta t u``,
-  METIS_TAC [dpm_is_perm, nomsetTheory.is_perm_inverse, eta_dpm]);
+  METIS_TAC [nomsetTheory.pmact_inverse, eta_dpm]);
 
 val alt_eta_redex = prove(
   ``~(0 IN dFV t) ==> eta (dABS (dAPP t (dV 0))) (nsub u 0 t)``,
